clean up

kalloc/clients.c
@@ -9,7 +9,7 @@ struct struct_kmem {
   struct run *freelist; 
 } kmem;
 
-void kfree1(void *pa) 
+void kfree(void *pa) 
 {
   struct run *r;
   r = (struct run*)pa;
@@ -20,7 +20,7 @@ void kfree1(void *pa)
   
 }
 
-void *kalloc1(void) 
+void *kalloc(void) 
 {
   struct run *r;
   r = kmem.freelist;
@@ -32,33 +32,33 @@ void *kalloc1(void)
 // not added to client 1 yet -- it is in simple-kfree
 void freerange_while_loop(void *pa_start, void *pa_end) {  // admit on pointer
   while ((char*)pa_start + PGSIZE <= (char*)pa_end) { 
-      kfree1(pa_start);
+      kfree(pa_start);
       pa_start = (char*)pa_start + PGSIZE;
   }
 }
 
 // should return pa
 void *client1(void *pa) {
-  kfree1(pa);
-  return kalloc1();
+  kfree(pa);
+  return kalloc();
 }
 
 
 
 // should return pa1
 void *client2(void *pa1, void *pa2) {
-  kfree1(pa1);
-  kfree1(pa2);
-  kalloc1();
-  return kalloc1();
+  kfree(pa1);
+  kfree(pa2);
+  kalloc();
+  return kalloc();
 }
 
 
 // should return pa2
 void *client3(void *pa1, void *pa2) {
-  kfree1(pa1);
-  kfree1(pa2);
-  return kalloc1();
+  kfree(pa1);
+  kfree(pa2);
+  return kalloc();
 }
 
 void *client4(void *pa1, void *pa2) {
@@ -67,37 +67,37 @@ void *client4(void *pa1, void *pa2) {
 }
 
 void *client5(void *pa1, void *pa2) {
-  kfree1(pa1);
-  kalloc1();
-  kfree1(pa2);
-  return kalloc1();
+  kfree(pa1);
+  kalloc();
+  kfree(pa2);
+  return kalloc();
 }
 
 
 void *client6(void *pa_start) {
   int i = 0;
   while (i < 2) {
-      kfree1(pa_start);
+      kfree(pa_start);
       pa_start = (char*)pa_start + PGSIZE;
       i++;
   }
-  return kalloc1();
+  return kalloc();
 }
 
 void *client7(void *pa_start, int n) {
   int i = 0;
   while (i < n) {
-      kfree1(pa_start);
+      kfree(pa_start);
       pa_start = (char*)pa_start + PGSIZE;
       i++;
   }
-  return kalloc1();
+  return kalloc();
 }
 
 void client8(void *pa_start, int n) {
   int i = 0;
   while (i < n) {
-      kfree1(pa_start);
+      kfree(pa_start);
       pa_start = (char*)pa_start + PGSIZE;
       i++;
   }
@@ -106,13 +106,13 @@ void client8(void *pa_start, int n) {
 // this is basicly doing the same as client 7
 void* client9(void *pa_start, int n) {
   client8(pa_start, n);
-  return kalloc1();
+  return kalloc();
 }
 
 // this is allowed..
 void client10(void *pa_start) {
-  kfree1(pa_start);
-  kfree1(pa_start);
+  kfree(pa_start);
+  kfree(pa_start);
 }
 
 
@@ -136,7 +136,7 @@ void client_11_pipealloc()
   struct pipe *pi;
 
   pi = 0;
-  pi = (struct pipe*)kalloc1(); 
+  pi = (struct pipe*)kalloc(); 
   if(pi) {
     pi->readopen = 1;
     pi->writeopen = 1;
@@ -149,7 +149,7 @@ int client12_42(void) {
 
   int *pa;
   pa = 0;
-  pa = (int*)kalloc1();           // cast to int pointer
+  pa = (int*)kalloc();           // cast to int pointer
   if (pa) {
     *pa = 42;
     int X = *pa;
@@ -163,11 +163,11 @@ int client12_42_include_free(void) {
 
   int *pa;
   pa = 0;
-  pa = (int*)kalloc1();           // cast to int pointer
+  pa = (int*)kalloc();           // cast to int pointer
   if (pa) {
     *pa = 42;
     int X = *pa;
-    kfree1(pa);
+    kfree(pa);
     return X;
   }
   return 0;
