kalloc/kalloc.c
@@ -1,0 +1,53 @@
+// Physical memory allocator, for user processes,
+// kernel stacks, page-table pages,
+// and pipe buffers. Allocates whole 4096-byte pages.
+
+void freerange(void *pa_start, void *pa_end);
+
+extern char end[]; // first address after kernel.
+                   // defined by kernel.ld.
+
+struct run {
+  struct run *next;
+};
+
+struct {
+  int xx;
+  struct run *freelist;
+} kmem;
+
+/* void
+freerange(void *pa_start, void *pa_end)
+{
+  char *p;
+  p = (char*)PGROUNDUP((uint64)pa_start);
+  for(; p + PGSIZE <= (char*)pa_end; p += PGSIZE)
+    kfree(p);
+}
+ */
+
+// Free the page of physical memory pointed at by pa,
+// which normally should have been returned by a
+// call to kalloc().  (The exception is when
+// initializing the allocator; see kinit above.)
+void kfree(void *pa) 
+{
+  struct run *r;
+  r = (struct run*)pa;
+  if (r) {
+    r->next = kmem.freelist;
+    kmem.freelist = r;
+  }
+}
+
+// Allocate one 4096-byte page of physical memory.
+// Returns a pointer that the kernel can use.
+// Returns 0 if the memory cannot be allocated.
+void *kalloc(void)
+{
+  struct run *r;
+  r = kmem.freelist;
+  if(r)
+    kmem.freelist = r->next;
+  return (void*)r; 
+}
